examples/pseudo_bool/cp_encoding/cp_to_ilp_linearScript.sml
@@ -64,7 +64,7 @@ End
 
 Theorem encode_lin_equal_sem_1:
   valid_assignment bnd wi ∧
-  ALOOKUP cs name = SOME (Linear (Lin reif cmp cXs Y)) ∧
+  ALOOKUP cs name = SOME (Linear (Lin Zr Equal cXs Y)) ∧
   reify_sem Zr wi
     (eval_iclin_term wi cXs = varc wi Y) ⇒
   EVERY (λx. iconstraint_sem x (wi,reify_avar cs wi))
@@ -137,7 +137,7 @@ End
 
 Theorem encode_lin_not_equal_sem_1:
   valid_assignment bnd wi ∧
-  ALOOKUP cs name = SOME (Linear (Lin reif cmp cXs Y)) ∧
+  ALOOKUP cs name = SOME (Linear (Lin Zr NotEqual cXs Y)) ∧
   reify_sem Zr wi
     (eval_iclin_term wi cXs ≠ varc wi Y) ⇒
   EVERY (λx. iconstraint_sem x (wi,reify_avar cs wi))
@@ -151,7 +151,7 @@ Proof
   intLib.ARITH_TAC
 QED
 
-Theorem encode_not_equal_sem_2:
+Theorem encode_lin_not_equal_sem_2:
   valid_assignment bnd wi ∧
   EVERY (λx. iconstraint_sem x (wi,wb))
     (encode_lin_not_equal bnd Zr cXs Y name) ⇒
@@ -170,35 +170,103 @@ Proof
   intLib.ARITH_TAC
 QED
 
+(* this encompasses ≥, >, ≤, < *)
+Definition encode_lin_cmp_aux_def:
+  encode_lin_cmp_aux cmp cXs Y =
+  case cmp of
+    GreaterEqual => mk_lin_ge cXs Y
+  | GreaterThan  => mk_lin_gt cXs Y
+  | LessEqual    => mk_lin_le cXs Y
+  | LessThan     => mk_lin_lt cXs Y
+  | _            => false_constr
+End
+
+Definition encode_lin_order_cmpops_def:
+  encode_lin_order_cmpops bnd Zr cmp cXs Y =
+  let constr = encode_lin_cmp_aux cmp cXs Y
+  in
+    case Zr of
+      NONE => [constr]
+    | SOME (INL Z) =>
+      encode_ge bnd Z 1 ++
+      [bits_imply bnd [Pos (INL (Ge Z 1))] constr]
+    | SOME (INR Z) =>
+      encode_ge bnd Z 1 ++
+      bimply_bits bnd [Pos (INL (Ge Z 1))] constr
+End
+
+Theorem encode_lin_order_cmpops_sem_1:
+  valid_assignment bnd wi ∧ cmp ≠ Equal ∧ cmp ≠ NotEqual ∧
+  reify_sem Zr wi (cmpop_val cmp (eval_iclin_term wi cXs) (varc wi Y)) ⇒
+  EVERY (λx. iconstraint_sem x (wi,reify_avar cs wi))
+    (encode_lin_order_cmpops bnd Zr cmp cXs Y)
+Proof
+  Cases_on ‘cmp’>>
+  rw[reify_sem_def,cmpop_val_def,
+    encode_lin_order_cmpops_def,
+    iconstraint_sem_def,encode_lin_cmp_aux_def]>>
+  every_case_tac>>
+  gvs[AllCasePreds(),reify_avar_def,reify_reif_def,
+    eval_iclin_term_CONS]>>
+  intLib.ARITH_TAC
+QED
+
+Theorem encode_lin_order_cmpops_sem_2:
+  valid_assignment bnd wi ∧ cmp ≠ Equal ∧ cmp ≠ NotEqual ∧
+  EVERY (λx. iconstraint_sem x (wi,wb))
+    (encode_lin_order_cmpops bnd Zr cmp cXs Y) ⇒
+  reify_sem Zr wi (cmpop_val cmp (eval_iclin_term wi cXs) (varc wi Y))
+Proof
+  rw[reify_sem_def,cmpop_val_def,
+    encode_lin_order_cmpops_def,encode_lin_cmp_aux_def]>>
+  every_case_tac>>
+  gvs[eval_iclin_term_CONS]>>
+  intLib.ARITH_TAC
+QED
+
 (* Linear constraint: Σ ci·Xi cmp Y *)
 Definition encode_lin_def:
-  encode_lin bnd Zr cmp Xs Y =
-  [false_constr]
+  encode_lin bnd Zr cmp cXs Y name =
+  if cmp = Equal
+  then encode_lin_equal bnd Zr cXs Y name
+  else if cmp = NotEqual
+  then encode_lin_not_equal bnd Zr cXs Y name
+  else encode_lin_order_cmpops bnd Zr cmp cXs Y
 End
 
 Theorem encode_lin_sem_1:
   valid_assignment bnd wi ∧
-  ALOOKUP cs name = SOME (Linear (Lin Zr cmp Xs Y)) ∧
-  lin_sem Zr cmp Xs Y wi ⇒
+  ALOOKUP cs name = SOME (Linear (Lin Zr cmp cXs Y)) ∧
+  lin_sem Zr cmp cXs Y wi ⇒
   EVERY (λx. iconstraint_sem x (wi,reify_avar cs wi))
-    (encode_lin bnd Zr cmp Xs Y)
+    (encode_lin bnd Zr cmp cXs Y name)
 Proof
-  cheat
+  rw[encode_lin_def,lin_sem_def]
+  >-gs[encode_lin_equal_sem_1,cmpop_val_def]
+  >-gs[encode_lin_not_equal_sem_1,cmpop_val_def]>>
+  metis_tac[encode_lin_order_cmpops_sem_1]
 QED
 
 Theorem encode_lin_sem_2:
   valid_assignment bnd wi ∧
   EVERY (λx. iconstraint_sem x (wi,wb))
-    (encode_lin bnd Zr cmp Xs Y) ⇒
-  lin_sem Zr cmp Xs Y wi
+    (encode_lin bnd Zr cmp cXs Y name) ⇒
+  lin_sem Zr cmp cXs Y wi
 Proof
-  cheat
+  rw[encode_lin_def,lin_sem_def]
+  >-(
+    simp[cmpop_val_def]>>
+    metis_tac[encode_lin_equal_sem_2])
+  >-(
+    simp[cmpop_val_def]>>
+    metis_tac[encode_lin_not_equal_sem_2])>>
+  metis_tac[encode_lin_order_cmpops_sem_2]
 QED
 
 Definition encode_linear_constr_def:
   encode_linear_constr bnd c name =
-  case c of Lin Zr cmp Xs Y =>
-    encode_lin bnd Zr cmp Xs Y
+  case c of Lin Zr cmp cXs Y =>
+    encode_lin bnd Zr cmp cXs Y name
 End
 
 Theorem encode_linear_constr_sem_1:
@@ -297,9 +365,65 @@ Proof
   simp[]
 QED
 
+Definition cencode_lin_order_cmpops_def:
+  cencode_lin_order_cmpops bnd Zr cmp cXs Y name ec =
+  let constr = encode_lin_cmp_aux cmp cXs Y
+  in
+    case Zr of
+      NONE =>
+      (List [
+        (SOME (strlit"c[" ^ name ^ strlit"]"), constr)], ec)
+    | SOME (INL Z) =>
+      let
+        (e,ec') = cencode_ge bnd Z 1 ec
+      in
+      (Append e $
+        List [
+        (SOME (strlit"c[" ^ name ^ strlit"]"),
+          (bits_imply bnd [Pos (INL (Ge Z 1))] constr))], ec')
+    | SOME (INR Z) =>
+      let
+        (e,ec') = cencode_ge bnd Z 1 ec
+      in
+      (Append e $
+        List (mk_annotate
+        [strlit"c[" ^ name ^ strlit"][r]";
+          strlit"c[" ^ name ^ strlit"][f]"]
+        (bimply_bits bnd [Pos (INL (Ge Z 1))] constr)), ec')
+End
+
+Theorem cencode_lin_order_cmpops_sem:
+  valid_assignment bnd wi ∧
+  cencode_lin_order_cmpops bnd Zr cmp cXs Y name ec = (es, ec') ⇒
+  enc_rel wi es (encode_lin_order_cmpops bnd Zr cmp cXs Y) ec ec'
+Proof
+  rw[cencode_lin_order_cmpops_def,encode_lin_order_cmpops_def]>>
+  gvs[AllCaseEqs(),UNCURRY_EQ]
+  >- (
+    irule enc_rel_abstr_cong>>
+    simp[])
+  >- (
+    irule enc_rel_Append>>
+    irule_at Any enc_rel_encode_ge>>
+    simp[]>>
+    irule enc_rel_abstr_cong>>
+    simp[])
+  >- (
+    irule enc_rel_Append>>
+    irule_at Any enc_rel_encode_ge>>
+    simp[]>>
+    irule enc_rel_List_mk_annotate)
+QED
+
 Definition cencode_linear_constr_def:
   cencode_linear_constr bnd c name ec =
-  (List [], ec)
+  case c of
+    Lin Zr cmp cXs Y =>
+      if cmp = Equal
+      then cencode_lin_equal bnd Zr cXs Y name ec
+      else if cmp = NotEqual
+      then cencode_lin_not_equal bnd Zr cXs Y name ec
+      else cencode_lin_order_cmpops bnd Zr cmp cXs Y name ec
 End
 
 Theorem cencode_linear_constr_sem:
@@ -307,5 +431,10 @@ Theorem cencode_linear_constr_sem:
   cencode_linear_constr bnd c name ec = (es, ec') ⇒
   enc_rel wi es (encode_linear_constr bnd c name) ec ec'
 Proof
-  cheat
+  Cases_on ‘c’>>
+  rename1 ‘Lin Zr cmp cXs Y’>>
+  rw[cencode_linear_constr_def,encode_linear_constr_def,encode_lin_def]
+  >-simp[cencode_lin_equal_sem]
+  >-simp[cencode_lin_not_equal_sem]>>
+  metis_tac[cencode_lin_order_cmpops_sem]
 QED
